CP in adding lemmas for bind to compose high and low state

examples/refinement/LowComp.fst
@@ -27,14 +27,32 @@ let well_formed h = fun (r1, r2) -> live h r1 /\ live h r2 /\ disjoint r1 r2
 val lstate_as_state : HS.mem -> lstate -> GTot state
 let lstate_as_state h  = fun (b1, b2) -> (B.get h b1 0, B.get h b2 0)
 
-
-
 val state_as_lstate : h:HS.mem -> ls:lstate{well_formed h ls} -> state -> GTot HS.mem 
 let state_as_lstate h =
   fun (r1, r2) (v1, v2) ->
     let h' = g_upd r1 0 v1 h in
     let p = g_upd_preserves_live h r1 r2 v1 in
     g_upd r2 0 v2 h'
+
+
+val state_as_lstate_inv : h:HS.mem -> ls:lstate{well_formed h ls} -> bs:state ->
+   Lemma (let h' = state_as_lstate h ls bs in 
+          lstate_as_state h' ls = bs)
+let state_as_lstate_inv h ls bs = 
+  let (b1, b2) = ls in 
+  let (s1, s2) = bs in
+  let h1 = g_upd b1 0 s1 h in 
+  let l1 = g_upd_preserves_live h b1 b2 s1 in
+  let h2 = g_upd b2 0 s2 h1 in
+  let l2 = g_upd_preserves_live h1 b2 b1 s2 in
+    
+  let p1 = get_upd_same h b1 s1 in  
+  assert (get h1 b1 0 == s1);
+  let p1' = get_upd_other h1 b2 b1 s2 s1 in
+  assert (get h2 b1 0 == get h1 b1 0); 
+  let p2 = get_upd_same h1 b2 s2 in
+  assert (get h2 b2 0 == s2);
+  ()
 
 // Low type variations
 
@@ -63,6 +81,18 @@ let lcomp_wp1 (a:Type) (wp : state -> (a * state -> Type) -> Type) (c : comp_wp 
                      (let tls = state_as_lstate h ls in // XXX fails otherwise
                       let (x, s1) = c s0 in 
                       h' == tls s1 /\ x == r ))))
+
+let lcomp_wp2 (a:Type) (wp : state -> (a * state -> Type) -> Type) (c : comp_wp a wp) =
+     (ls:lstate) ->
+     Stack a
+       (requires (fun h -> well_formed h ls))
+       (ensures  (fun h r h' ->
+                    well_formed h' ls /\
+                    (let s0 = lstate_as_state h ls in
+                      wp s0 (fun _ -> True) ==> 
+                      (let tls = state_as_lstate h ls in // XXX fails otherwise
+                       let (x, s1) = c s0 in 
+                       h' == tls s1 /\ x == r ))))
 
 
 // This is the variation currenlty used
@@ -133,17 +163,23 @@ let lreturn (#a:Type) (x:a) : lcomp_wp1 a (return_wp x) (hreturn' x) =
     let p2 = get_upd_eq h0 b2 0 (get h0 b2 0) in
     x
 
+
+// Not sure why this doesn't verify. Result type should follow from the assertions
 val lwrite : i:nat{ i < 2 } -> v:mint -> lcomp_wp1 unit (write_wp i v) (hwrite' i v)
 let lwrite i v = fun (b1, b2) -> 
+   let h0 = ST.get () in
     if i = 0 then 
-      let h0 = ST.get () in
-      let h1 = g_upd b1 v h0 in
-      let p = get_upd_other h0 b2 b1 (get h0 b2 0) v in
-      let p2 = get_upd_eq (g_upd b1 0 v h0) b2 0 (get h0 b2 0) in
+      let p = 
+        let p = g_upd_preserves_live h0 b1 b2 v in // Shows: live h1 b
+        let g = get_upd_other h0 b1 b2 v (get h0 b2 0) in // Shows: get (g_upd b1 v h0) b2 = get h0 b2 
+        assert (get (g_upd b1 0 v h0) b2 0 == get h0 b2 0);
+        get_upd_eq (g_upd b1 0 v h0) b2 0 (get h0 b2 0) // Shows: g_upd b2 0 (get h0 b2 0) h1 == h1
+      in
+      assert (g_upd b2 0 (get h0 b2 0) (g_upd b1 0 v h0) == g_upd b1 0 v h0);
       b1.(0ul) <- v 
     else 
-      let h0 = ST.get () in 
       let p1 = get_upd_eq h0 b1 0 (get h0 b1 0) in
+      assert (g_upd b2 0 v (g_upd b1 0 (get h0 b1 0) h0) == g_upd b2 0 v h0);
       b2.(0ul) <- v
 
 val lread : i:nat{ i < 2 } -> lcomp_wp1 mint (read_wp i) (hread' i)
@@ -165,9 +201,22 @@ let lbind (#a:Type) (#b:Type)
   (#c1:comp_wp a wp1) (#c2:(x:a -> comp_wp b (wp2 x)))
   (m: lcomp_wp a wp1 c1) (f: (x:a) -> lcomp_wp b (wp2 x) (c2 x)):
   lcomp_wp b (bind_wp wp1 wp2) (hbind' c1 c2) =
-  fun s ->
+  fun ls ->
     assume (monotonic wp1);
-    let a = m s in let r = f a s in r
+    let h0 = ST.get () in 
+    let a = m ls in 
+    let h1 = ST.get () in
+
+    let p = 
+       let (r, s1) = c1 (lstate_as_state h0 ls) in
+       state_as_lstate_inv h0 ls s1 
+    in
+    // assert (let s0 = lstate_as_state h0 ls in
+    //         let (r, s1) = c1 s0 in
+    //         let h1' = state_as_lstate h0 ls s1 in 
+    //         lstate_as_state h1' ls == s1);
+            
+    let r = f a ls in r
 
 
 // Versions of [lread] and [lwrite] with reif in spec
@@ -175,12 +224,8 @@ let lbind (#a:Type) (#b:Type)
 val lwrite' : i:nat{ i < 2 } -> v:mint -> lcomp_wp unit (write_wp i v) (reify (HIGH?.put i v))
 let lwrite' i v = fun (b1, b2) -> 
   if i = 0 then 
-    let h0 = ST.get () in 
-    let p1 = get_upd_eq h0 b1 0 (get h0 b1 0) in
-    let p2 = get_upd_eq h0 b2 0 (get h0 b2 0) in
     b1.(0ul) <- v 
-  else 
-    
+  else     
     b2.(0ul) <- v
 
 val lread' : i:nat{ i < 2 } -> lcomp_wp1 mint (read_wp i) (reify (HIGH?.get i))
@@ -190,13 +235,8 @@ let lread' i = fun (b1, b2) ->
   let p2 = get_upd_eq h0 b2 0 (get h0 b2 0) in
   if i = 0 then b1.(0ul) else b2.(0ul)
 
-// 
 
 let lcomp_respects_h_eq (a : Type) (wp1 : hwp a) (wp2 : hwp a) (hc1 : comp_wp a wp1) (hc2 : comp_wp a wp2)  
-  (lc : lcomp_wp a wp1 hc1) (p : h_eq wp1 wp2 hc1 hc2) : lcomp_wp' a wp2 hc2 = //660 requires the lcomp_wp'
-   // assert (forall s0. wp1 s0 (fun _ -> True) <==> wp2 s0 (fun _ -> True));
-   // assert (forall s0. wp2 s0 (fun _ -> True) ==> 
-   //               wp1 s0 (fun _ -> True) /\
-   //               hc1 s0 == hc2 s0);      
+  (lc : lcomp_wp a wp1 hc1) (p : h_eq wp1 wp2 hc1 hc2) : lcomp_wp' a wp2 hc2 = // 660 requires the lcomp_wp'
    lc 
   
