examples/refinement/Mem_eq.fst
@@ -31,8 +31,14 @@ val upd_upd_eq : #a:Type -> h:mem -> b:pointer a{live h b} -> i:nat{i < length b
 let upd_upd_eq #a h i b v1 v2 = admit ()
 
 
+val get_upd_same : #a:Type -> h:mem -> b1:pointer a{live h b1} -> v1:a ->
+    Lemma (get (g_upd b1 0 v1 h) b1 0 == v1)
+let get_upd_same #a h b1 v1 = admit ()
 
-val get_upd_other : #a:Type -> h:mem -> b1:pointer a{live h b1} -> b2:pointer a{live h b2} -> v1:a -> v2:a ->
+
+
+val get_upd_other : #a:Type -> h:mem -> b1:pointer a{live h b1} -> b2:pointer a{live h b2} -> 
+    v1:a -> v2:a ->
     Lemma (requires (get h b2 0 == v2 /\ disjoint b1 b2))
           (ensures (get (g_upd b1 0 v1 h) b2 0 == v2))
 let get_upd_other #a h b1 b2 v1 v2 = admit ()
